src/graph_theory/path_embedding.lean
@@ -6,10 +6,10 @@ namespace simple_graph
 
     structure path_embedding (G : simple_graph V) (G' : simple_graph V') :=
         (f        : V ↪ V')
-        (df       : Π e : edges G, path G' (f e.x) (f e.y))
+        (df       : Π e : edge G, path G' (f e.x) (f e.y))
         --
-        (nodup    : ∀ e : edges G, (df e).nodup)
-        (sym      : ∀ e : edges G, df e.flip = (df e).rev)
+        (nodup    : ∀ e : edge G, (df e).nodup)
+        (sym      : ∀ e : edge G, df e.flip = (df e).rev)
         --
         (endpoint : ∀ {e x},    f x ∈ df e              -> x ∈ e.ends)
         (disjoint : ∀ {e e' z},   z ∈ df e -> z ∈ df e' -> e.ends = e'.ends ∨ ∃ x, z = f x)
@@ -19,7 +19,7 @@ namespace simple_graph
     namespace path_embedding
         variables {G : simple_graph V} {G' : simple_graph V'} (F : path_embedding G G') {x y z : V}
 
-        lemma nop {e : edges G} : 0 < (F.df e).size
+        lemma nop {e : edge G} : 0 < (F.df e).size
             := by {
                 cases nat.eq_zero_or_pos (F.df e).size, swap, exact h, exfalso,
                 exact G.ne_of_adj e.h (F.f.injective (path.point_of_size_0 h))
@@ -101,7 +101,7 @@ namespace simple_graph
                     replace h3 := path.mem_edges h3,
                     replace h5 := path.mem_edges h5,
                     replace h5 : e1.x ∈ F.df e' ∧ e1.y ∈ F.df e' := by {
-                        cases edges.same_iff.mpr h7; subst e2,
+                        cases edge.same_iff.mpr h7; subst e2,
                         exact h5, simp at h5, exact h5.symm
                     }, clear h7,
                     cases F.disjoint h3.1 h5.1 with h10 h10, exact h10,
@@ -113,7 +113,7 @@ namespace simple_graph
                     have h14 := F.endpoint h5.1,
                     have h15 := F.endpoint h5.2,
                     have h16 : x ≠ y := by { intro h, apply G'.ne_of_adj e1.h, convert congr_arg F.f h },
-                    exact edges.sym2_eq h16 h12 h13 h14 h15
+                    exact edge.sym2_eq h16 h12 h13 h14 h15
                 },
                 {
                     obtain ⟨y,h8⟩ := h7, subst z,
@@ -121,8 +121,8 @@ namespace simple_graph
                     replace h6 := F'.endpoint h6,
                     replace h3 := path.mem_edges h3,
                     replace h5 := path.mem_edges h5,
-                    replace h3 : y ∈ F.df e, by { cases edges.mem_edge.mp h4; subst h, exact h3.1, exact h3.2 },
-                    replace h5 : y ∈ F.df e', by { cases edges.mem_edge.mp h6; subst h, exact h5.1, exact h5.2 },
+                    replace h3 : y ∈ F.df e, by { cases edge.mem_edge.mp h4; subst h, exact h3.1, exact h3.2 },
+                    replace h5 : y ∈ F.df e', by { cases edge.mem_edge.mp h6; subst h, exact h5.1, exact h5.2 },
                     cases F.disjoint h3 h5 with h9 h9,
                         { left, exact h9 },
                         { obtain ⟨x,h9⟩ := h9, subst h9, right, use x, refl }
